FEC/Verif_matrix.v
@@ -9,6 +9,7 @@ Require Import Specs.
 Require Import FECTactics.
 Require Import ByteFacts.
 Require Import ByteField.
+Require Import VandermondeByte.
 
 Set Bullet Behavior "Strict Subproofs".
 (*
@@ -17,147 +18,110 @@ Set Bullet Behavior "Strict Subproofs".
 Lemma body_rse_init : semax_body Vprog Gprog f_rse_init rse_init_spec.
 Proof.
   start_function. forward_call. forward_call. entailer!.
-Qed.
+Qed.*)
+
+(*TODO: move*)
+(*Need because "forward" gives some weird defaults for Znth*)
+Lemma Znth_default: forall {A: Type} (H2 H1: Inhabitant A) (l: list A) (i: Z),
+  0 <= i < Zlength l ->
+  @Znth _ H1 i l = @Znth _ H2 i l.
+Proof.
+  intros A Hin1 Hin2 l i Hi. unfold Znth. destruct (zlt i 0); try lia.
+  apply nth_indep. rewrite <-ZtoNat_Zlength. lia.
+Qed. 
 
 (** Verification of [fec_generate_weights]*)
 Lemma body_fec_generate_weights : semax_body Vprog Gprog f_fec_generate_weights fec_generate_weights_spec.
 Proof.
-  pose proof (mod_poly_PosPoly) as Hpospoly.
-  pose proof (mod_poly_PrimPoly) as Hprimpoly.
-  start_function. freeze Ftrace := (data_at _ _ _ (gv _trace)).
-    forward_loop (EX (i : Z) (l: list (list Z)),
-    PROP (0 <= i <= fec_max_h; Zlength l = fec_max_h; Forall (fun x => Zlength x = fec_n - 1) l;
-        forall (x: Z), 0 <= x < i -> (forall (y: Z), 0 <= y < fec_n - 1 -> Znth y (Znth x l) = 
-        poly_to_int ((monomial (Z.to_nat (x * y)) %~ mod_poly ))))
-    LOCAL (gvars gv; temp _i (Vint (Int.repr i)))
-    SEP (FRZL Ftrace; FIELD_TABLES gv;
-        data_at Ews (tarray (tarray tuchar (fec_n - 1)) fec_max_h) (map_int_val_2d l) (gv _fec_weights)))
-    break:
-      (PROP ()
-      LOCAL (gvars gv)
-      SEP (data_at Ews tint (Vint (Int.zero)) (gv _trace); FIELD_TABLES gv;
-          data_at Ews (tarray (tarray tuchar (fec_n - 1)) fec_max_h) 
-          (rev_mx_val (weight_mx_list fec_max_h (fec_n - 1)))  (gv _fec_weights))). 
-  - forward. Exists 0%Z. Exists (list_repeat (Z.to_nat fec_max_h) (list_repeat (Z.to_nat (fec_n - 1)) 0%Z)).
-    entailer!. split. rewrite Zlength_list_repeat'. rep_lia. rewrite Forall_forall. intros x Hin.
-    apply in_list_repeat in Hin. subst. rewrite Zlength_list_repeat'. rep_lia. unfold map_int_val_2d. unfold map_2d.
-    rewrite !map_list_repeat. cancel. 
-  - Intros i. Intros l. forward_if.
-    + forward_loop (EX (j : Z) (l: list (list Z)),
-         PROP (0 <= j <= fec_n - 1; Zlength l = fec_max_h; Forall (fun x => Zlength x = fec_n - 1) l;
-      (forall (x y: Z), (0 <= x < i /\ 0 <= y < fec_n - 1) \/ (x = i /\ 0 <= y < j) -> Znth y (Znth x l) = 
-        poly_to_int ((monomial (Z.to_nat (x * y)) %~ mod_poly ))))
+  (*pose proof (mod_poly_PosPoly) as Hpospoly.
+  pose proof (mod_poly_PrimPoly) as Hprimpoly.*)
+ start_function. freeze Ftrace := (data_at _ _ _ (gv _trace)).
+ forward_loop (EX (i : Z),
+  PROP (0 <= i <= fec_max_h)
+  LOCAL (gvars gv; temp _i (Vint (Int.repr i)))
+  SEP (FRZL Ftrace; FIELD_TABLES gv;
+        data_at Ews (tarray (tarray tuchar (fec_n - 1)) fec_max_h) 
+          (mx_val (pop_weight_mx i 0)) (gv _fec_weights)))
+  break: (PROP ()
+    LOCAL (gvars gv)
+    SEP (data_at Ews tint (Vint (Int.zero)) (gv _trace); FIELD_TABLES gv;
+        data_at Ews (tarray (tarray tuchar (fec_n - 1)) fec_max_h) 
+        (rev_mx_val (weight_mx_list fec_max_h (fec_n - 1)))  (gv _fec_weights))). 
+{ forward. entailer!. Exists 0. entailer!. rewrite pop_weight_mx_zero. rewrite mx_val_zseq. cancel. } 
+{ Intros i. forward_if.
+  { forward_loop (EX (j: Z), 
+      PROP (0 <= j <= fec_n - 1)
       LOCAL (gvars gv; temp _i (Vint (Int.repr i)); temp _j (Vint (Int.repr j)))
       SEP (FRZL Ftrace; FIELD_TABLES gv;
-           data_at Ews (tarray (tarray tuchar (fec_n - 1)) fec_max_h) (map_int_val_2d l) (gv _fec_weights)))
-      break: (EX (l: list (list Z)),
-        (PROP (Zlength l = fec_max_h; Forall (fun x => Zlength x = fec_n - 1) l;
-          forall (x: Z), 0 <= x <= i -> (forall (y: Z), 0 <= y < fec_n - 1 -> Znth y (Znth x l) = 
-          poly_to_int ((monomial (Z.to_nat (x * y)) %~ mod_poly ))))
-        LOCAL (gvars gv; temp _i (Vint (Int.repr i)))
-        SEP (FRZL Ftrace; FIELD_TABLES gv;
-             data_at Ews (tarray (tarray tuchar (fec_n - 1)) fec_max_h) (map_int_val_2d l) (gv _fec_weights)))).
-      * forward. Exists 0%Z. Exists l. entailer!. intros x y [Hbefore | Hcont]. apply H2; lia. lia.
-      * Intros j. Intros lj. forward_if.
-        -- (*Want to simplify the index*)
-            assert (Hprod: 0 <= (i * j) mod 255 < fec_n). {  pose proof (Z.mod_pos_bound (i * j) 255). rep_lia. }
-            assert (Hidx : Int.signed (Int.mods (Int.repr (i * j)) (Int.repr 255)) = (i * j) mod 255). {
-              assert (Int.min_signed <= i * j <= Int.max_signed). {
-              split. rep_lia. assert (i * j <= fec_max_h * (fec_n - 1)).
-              apply Z.mul_le_mono_nonneg; lia. assert (fec_max_h * (fec_n - 1) = 32640). rewrite fec_max_h_eq.
-              rewrite fec_n_eq. reflexivity. rep_lia. }
-              unfold Int.mods. rewrite !Int.signed_repr; try rep_lia. rewrite Z.rem_mod_nonneg by rep_lia.
-              reflexivity. rewrite !Int.signed_repr by rep_lia. pose proof (Z.rem_bound_pos_pos (i * j) 255). rep_lia. }
-            unfold FIELD_TABLES. unfold INDEX_TABLES. Intros.
-            forward.
-          ++ entailer!. simpl. rewrite Hidx. assumption. 
-          ++ entailer!. rewrite Hidx. rewrite power_to_index_contents_Znth. simpl. simpl_repr. rep_lia.         
-          ++ entailer!. (*Why do I get this goal?*)
-             destruct H23. apply repr_inj_signed in H24;  rep_lia.
-          ++ simpl. rewrite Hidx. rewrite power_to_index_contents_Znth; [| assumption]. 
-             assert_PROP (force_val  (sem_add_ptr_int tuchar Signed
-              (force_val (sem_add_ptr_int (tarray tuchar 255) Signed (gv _fec_weights) (Vint (Int.repr i))))
-              (Vint (Int.repr j))) = field_address (tarray (tarray tuchar (fec_n - 1)) fec_max_h)  
-                [ArraySubsc j; ArraySubsc i] (gv _fec_weights)).
-              { entailer!. solve_offset. }
-             forward. simpl_repr. forward.
-             Exists (j+1). Exists (upd_Znth i lj  (upd_Znth j (Znth i lj)
-              (poly_to_int (monomial (Z.to_nat ((i * j) mod 255)) %~ mod_poly)))). entailer!. (*inner loop re establish invariant*)
-            ** repeat split.
-              --- rewrite upd_Znth_Zlength. auto. rep_lia.
-              --- rewrite Forall_Znth. intros i' Hi'. rewrite Zlength_upd_Znth in Hi'.
-                  assert (Hii': i = i' \/ i <> i') by lia.
-                  destruct Hii' as [Hii' | Hneq]. subst. rewrite upd_Znth_same. 2: rep_lia.
-                  rewrite Zlength_upd_Znth. inner_length. rewrite upd_Znth_diff; try lia. inner_length. rep_lia.
-              --- intros x y [Hbef | Hcurr]. rewrite upd_Znth_diff by rep_lia. apply H7; lia.
-                  destruct Hcurr as [H' Hy]. subst. rewrite upd_Znth_same by rep_lia.
-                  assert (Hycase: 0 <= y < j \/ y = j) by lia.
-                  assert (Hlen: Zlength (Znth i lj) = fec_n - 1) by inner_length. 
-                  destruct Hycase as [Hbefore | Hcurr].
-                  rewrite upd_Znth_diff by rep_lia. apply H7; lia. 
-                  subst. rewrite upd_Znth_same by rep_lia. f_equal. apply (@monomial_powers_eq_mod _ _ Hprimpoly).
-                  rewrite Zmod_mod by lia. assert (Hfsz: Z.to_nat 255 = field_size mod_poly). {
-                  apply Nat2Z.inj. rewrite field_size_fec_n. rep_lia. } rewrite Hfsz. apply Nat.mod_mod; lia.
-              --- solve_repr_int. 
-            ** unfold map_int_val_2d. unfold map_2d. rewrite <- !upd_Znth_map. rewrite !Znth_map. entailer!.
-               rep_lia.
-        -- (*end of inner loop*) forward. Exists lj. entailer!. intros x Hx y Hy.
-           apply H7. rep_lia.
-      * Intros lj. forward. Exists (i+1)%Z. Exists lj. entailer!. split.
-        -- intros x Hx y Hy. apply H6; lia.
-        -- solve_repr_int. 
-    + (*end of outer loop*) forward. entailer!.
-      assert (Hweight: (map_int_val_2d l) = (rev_mx_val (weight_mx_list fec_max_h (fec_n - 1)))). {
-      unfold rev_mx_val. unfold map_int_val_2d. unfold rev_mx. unfold map_2d. unfold map_2d_rev. rewrite !map_map.
-      apply Znth_eq_ext.
-        - rewrite !Zlength_map. unfold weight_mx_list. unfold mk_matrix; rewrite prop_list_length. lia. rep_lia.
-        - intros i' Hi'. rewrite Zlength_map in Hi'. rewrite H0 in Hi'.
-          assert (Hfn: 0 <= fec_n - 1) by rep_lia. assert (Hfh: 0 <= fec_max_h) by rep_lia. 
-          pose proof (weight_matrix_wf Hfn Hfh) as Hwf.
-          destruct Hwf as [Hlen [Hn Hinlen]]. 
-          rewrite !Znth_map;[ | | list_solve]. f_equal. f_equal.
-          unfold weight_mx_list. unfold mk_matrix; rewrite prop_list_Znth by rep_lia.
-          apply Znth_eq_ext.
-          + rewrite Zlength_rev. rewrite Zlength_map. rewrite prop_list_length. inner_length. rep_lia. 
-          + intros j' Hj'. assert (0 <= j' < fec_n - 1) by (revert Hj'; inner_length).
-            rewrite Znth_rev; rewrite !Zlength_map; rewrite !prop_list_length; try rep_lia.
-            rewrite !Znth_map; [ | rewrite prop_list_length; rep_lia].
-            rewrite prop_list_Znth by rep_lia. rewrite H2 by rep_lia. simpl. repeat f_equal. lia.
-          + simpl in *. rep_lia. }
-      rewrite Hweight. cancel. thaw Ftrace. cancel. 
-  - forward. forward_if True. contradiction. forward. entailer!.
-    assert (Hfn: 0 <= fec_n - 1) by rep_lia. assert (Hfh: 0 <= fec_max_h) by rep_lia. 
-    pose proof (weight_matrix_wf Hfn Hfh) as Hwf. assert (Hwf' := Hwf).
-    destruct Hwf' as [Hlen [Hn Hinlen]].
-    forward_call(gv, fec_max_h, fec_n - 1,  (weight_mx_list fec_max_h (fec_n - 1)),
+        data_at Ews (tarray (tarray tuchar (fec_n - 1)) fec_max_h) 
+         (mx_val (pop_weight_mx i j)) (gv _fec_weights)))
+     break: (PROP ()
+       LOCAL (gvars gv; temp _i (Vint (Int.repr i)))
+       SEP (FRZL Ftrace; FIELD_TABLES gv;
+        data_at Ews (tarray (tarray tuchar (fec_n - 1)) fec_max_h) 
+          (mx_val (pop_weight_mx (i + 1) 0)) (gv _fec_weights))).
+    { forward. Exists 0. entailer!. }
+    { Intros j. forward_if.
+      { assert (Hprod: 0 <= (i * j) mod 255 < fec_n). {  pose proof (Z.mod_pos_bound (i * j) 255). rep_lia. }
+        assert (Hidx : Int.signed (Int.mods (Int.repr (i * j)) (Int.repr 255)) = (i * j) mod 255). {
+          assert (Int.min_signed <= i * j <= Int.max_signed). {
+            split. rep_lia. assert (i * j <= fec_max_h * (fec_n - 1)).
+            apply Z.mul_le_mono_nonneg; lia. rep_lia.  } 
+          unfold Int.mods. rewrite !Int.signed_repr; try rep_lia. apply Z.rem_mod_nonneg; rep_lia.
+          rewrite !Int.signed_repr by rep_lia. pose proof (Z.rem_bound_pos_pos (i * j) 255). rep_lia. }
+        unfold FIELD_TABLES. unfold INDEX_TABLES. Intros. forward.
+        { entailer!. simpl. rep_lia. }
+        { entailer!. simpl_repr_byte. }
+        { entailer!. destruct H17. apply repr_inj_signed in H18; rep_lia. }
+        { simpl. rewrite Hidx. rewrite Znth_map by ( rewrite byte_pows_Zlength; rep_lia).
+          assert_PROP (force_val  (sem_add_ptr_int tuchar Signed
+            (force_val (sem_add_ptr_int (tarray tuchar 255) Signed (gv _fec_weights) (Vint (Int.repr i))))
+            (Vint (Int.repr j))) = field_address (tarray (tarray tuchar (fec_n - 1)) fec_max_h)  
+             [ArraySubsc j; ArraySubsc i] (gv _fec_weights)).
+            { entailer!. solve_offset. }
+          forward. simpl_repr_byte. rewrite <- (byte_int_repr (Byte.unsigned _)) by rep_lia.
+          rewrite Byte.repr_unsigned. forward. Exists (j+1). entailer!.
+          { simpl_repr_byte. }
+          { rewrite byte_pows_Znth by rep_lia. pose proof (pop_weight_mx_wf i j) as [Hlen _]. 
+            rewrite !(Znth_default Inhabitant_list). 2 : { rewrite mx_val_length1. rep_lia. }
+            rewrite (mx_val_upd_Znth) by rep_lia. rewrite pop_weight_mx_set by rep_lia. cancel. 
+          }
+        }
+      }
+      { forward. entailer!. replace j with (fec_n - 1) by rep_lia. rewrite pop_weight_mx_row_finish. cancel. }
+    }
+    { forward. Exists (i +1). entailer!. simpl_repr_byte. }
+  }
+  { forward. replace i with (fec_max_h) by rep_lia. thaw Ftrace. entailer!. rewrite pop_weight_weight_done. cancel. }
+}
+{ forward. forward_if True; [contradiction | |].
+  { forward. entailer!. }
+  { forward_call(gv, fec_max_h, fec_n - 1,  (weight_mx_list fec_max_h (fec_n - 1)),
       (gv _fec_weights)).
-    + entailer!. simpl. f_equal. solve_repr_int. repeat(f_equal); rep_lia. 
-    +  (*need the result about 2d and 1d arrays*) unfold FIELD_TABLES.
-      rewrite data_at_2darray_concat. unfold rev_mx_val. unfold map_int_val_2d. rewrite <- map_map.
-      unfold map_2d. rewrite <- !concat_map. unfold flatten_mx. rewrite !map_map. cancel.
-      simpl_map2d. auto. rewrite Forall_Znth; simpl_map2d. rewrite Hlen. intros i Hi.
-      simpl_map2d. rewrite Forall_Znth in Hinlen. apply Hinlen. lia. auto. 
-    + repeat(split; try rep_lia; auto).
+    { entailer!. simpl. simpl_repr_byte. rewrite !byte_int_repr by rep_lia. repeat f_equal; rep_lia. }
+    { assert(Hwf: wf_lmatrix (F:=B) (weight_mx_list fec_max_h (fec_n - 1)) fec_max_h (fec_n - 1)) by
+        (apply (@weight_matrix_wf fec_max_h (fec_n - 1)); rep_lia).
+      pose proof (rev_mx_val_wf _ _ _ Hwf) as Hrev. rewrite data_at_2darray_concat; auto; try apply Hrev.
+      rewrite concat_rev_mx. cancel.
+    }
+    { split; [rep_lia | split; [ rep_lia | split]]. apply weight_matrix_wf; rep_lia.
       unfold strong_inv_list. destruct (range_le_lt_dec 0 0 fec_max_h ); try rep_lia.
       destruct (Z_le_lt_dec fec_max_h (fec_n - 1)); try rep_lia. rewrite weight_mx_list_spec by rep_lia.
-      apply Vandermonde.vandermonde_strong_inv.
-      apply (ssrbool.introT (ssrnat.leP)). rewrite <- field_size_fec_n. unfold field_size. lia.
-    + Intros vret. forward. forward_if. contradiction. forward. 
-      assert (Hwf': (wf_matrix (gauss_restrict_rows (F:=F) fec_max_h (fec_n - 1) 
-          (weight_mx_list fec_max_h (fec_n - 1))) fec_max_h (fec_n - 1))).
-      apply gauss_restrict_rows_wf; solve_wf. assert (Hwf'' := Hwf'). destruct Hwf'' as [Hlen' [Hn' Hinlen']].
-      entailer!.
-      (*need to go back 1D-> 2D array*)
-      rewrite data_at_2darray_concat.
-      * apply derives_refl'. f_equal. unfold flatten_mx. unfold rev_mx_val. unfold map_int_val_2d. unfold map_2d.
-        unfold rev_mx. unfold map_2d_rev. rewrite !concat_map. rewrite !map_map. f_equal. unfold weight_mx.
-        simpl. apply map_ext. intros. rewrite !map_map. reflexivity.
-      * simpl_map2d. apply weight_mx_wf.
-      * rewrite Forall_Znth. simpl_map2d. intros i Hi. simpl_map2d. pose proof weight_mx_wf as [Hwlen [? Hwinlen]]. 
-        inner_length.
-      * auto.
+      apply vandermonde_strong_inv. apply (ssrbool.introT (ssrnat.leP)). rep_lia. 
+    }
+    { Intros ret. forward. forward_if True; [ contradiction | |].
+      { forward. entailer!. }
+      { forward. entailer!. pose proof weight_mx_wf as Hwf. pose proof (rev_mx_val_wf _ _ _ Hwf) as Hrev.
+        rewrite data_at_2darray_concat; auto; try apply Hrev.
+        rewrite concat_rev_mx. unfold weight_mx. cancel.
+      }
+    }
+  }
+}
 Qed.
-      *)
+
+(** Verification of [fec_matrix_transform]*)
+
 
 (*For some reason it unfold [byte_inv] even though it shouldn't so we need separate lemma*)
 Lemma force_val_byte: forall (b: byte),
@@ -187,12 +151,9 @@ Lemma byte_xor_fold: forall b1 b2,
 Proof.
   intros b1 b2. unfold Byte.xor. rewrite Byte.unsigned_repr; [ reflexivity | apply byte_xor_size].
 Qed.
-  
 
 Opaque byte_inv.
 Opaque byte_mul.
-
-(** Verification of [fec_matrix_transform]*)
 
 Lemma body_fec_matrix_transform : semax_body Vprog Gprog f_fec_matrix_transform fec_matrix_transform_spec.
 Proof.
